src/arch/x64/X64.Memory_i_s.fsti
@@ -319,49 +319,26 @@ val valid_state_store_mem128: ptr:int -> v:quad32 -> s:state -> Lemma (
 
 //Memtaint related functions
 
-val memtaint: Type u#0
+type memtaint = memTaint_t
 
-// TODO
-val correct_down_taint:(memTaint:memtaint) -> 
-                       (mem:mem) ->
-		       (bytesTaint:memTaint_t) ->
-		       Type0
-
-val down_taint: (memTaint:memtaint) -> 
-    	        (mem:mem) ->
-           GTot (bytesTaint:memTaint_t{correct_down_taint memTaint mem bytesTaint})
-
-val up_taint: (bytesTaint:memTaint_t) ->
-              (mem:mem) ->
-         GTot (memTaint:memtaint{correct_down_taint memTaint mem bytesTaint})
-
-val up_down_identity: (memTaint:memtaint) ->
-                      (mem:mem) ->
-	        Lemma (up_taint (down_taint memTaint mem) mem == memTaint)
-
-val down_up_identity: (bytesTaint:memTaint_t) ->
-                      (mem:mem) ->
-	        Lemma (down_taint (up_taint bytesTaint mem) mem == bytesTaint)
-
-
-val valid_taint_buf64 (b:buffer64) (memTaint:memtaint) (t:taint) : GTot Type0
-val valid_taint_buf128 (b:buffer128) (memTaint:memtaint) (t:taint) : GTot Type0
+val valid_taint_buf64 (b:buffer64) (mem:mem) (memTaint:memtaint) (t:taint) : GTot Type0
+val valid_taint_buf128 (b:buffer128) (mem:mem) (memTaint:memtaint) (t:taint) : GTot Type0
 
 val lemma_valid_taint64: (b:buffer64) ->
 			 (memTaint:memtaint) ->
 			 (mem:mem) ->
 			 (i:nat{i < buffer_length b}) ->
 			 (t:taint) -> Lemma
-  (requires valid_taint_buf64 b memTaint t /\ buffer_readable mem b)
-  (ensures Map.sel (down_taint memTaint mem) (buffer_addr b mem + 8 `op_Multiply` i) == t)
+  (requires valid_taint_buf64 b mem memTaint t /\ buffer_readable mem b)
+  (ensures Map.sel memTaint (buffer_addr b mem + 8 `op_Multiply` i) == t)
 
 val lemma_valid_taint128: (b:buffer128) ->
 			 (memTaint:memtaint) ->
 			 (mem:mem) ->
 			 (i:nat{i < buffer_length b}) ->
 			 (t:taint) -> Lemma
-  (requires valid_taint_buf128 b memTaint t /\ buffer_readable mem b)
-  (ensures Map.sel (down_taint memTaint mem) (buffer_addr b mem + 16 `op_Multiply` i) == t)
+  (requires valid_taint_buf128 b mem memTaint t /\ buffer_readable mem b)
+  (ensures Map.sel memTaint (buffer_addr b mem + 16 `op_Multiply` i) == t)
 
 val same_memTaint64: (b:buffer64) -> 
                    (mem0:mem) ->
@@ -369,7 +346,7 @@ val same_memTaint64: (b:buffer64) ->
 		   (memtaint0:memtaint) ->
 		   (memtaint1:memtaint) -> Lemma
   (requires (modifies (loc_buffer b) mem0 mem1 /\ 
-    (forall p. Map.sel (down_taint memtaint0 mem0) p == Map.sel (down_taint memtaint1 mem1) p)))
+    (forall p. Map.sel memtaint0 p == Map.sel memtaint1 p)))
   (ensures memtaint0 == memtaint1)
 
 val same_memTaint128: (b:buffer128) -> 
@@ -378,5 +355,19 @@ val same_memTaint128: (b:buffer128) ->
 		   (memtaint0:memtaint) ->
 		   (memtaint1:memtaint) -> Lemma
   (requires (modifies (loc_buffer b) mem0 mem1 /\ 
-    (forall p. Map.sel (down_taint memtaint0 mem0) p == Map.sel (down_taint memtaint1 mem1) p)))
+    (forall p. Map.sel memtaint0 p == Map.sel memtaint1 p)))
   (ensures memtaint0 == memtaint1)
+
+val modifies_valid_taint64 (b:buffer64) (p:loc) (h h':mem) (memTaint:memtaint) (t:taint) : Lemma
+  (requires
+    modifies p h h'
+  )
+  (ensures valid_taint_buf64 b h memTaint t <==> valid_taint_buf64 b h' memTaint t)
+  [SMTPat (modifies p h h'); SMTPat (valid_taint_buf64 b h' memTaint t)]
+
+val modifies_valid_taint128 (b:buffer128) (p:loc) (h h':mem) (memTaint:memtaint) (t:taint) : Lemma
+  (requires
+    modifies p h h'
+  )
+  (ensures valid_taint_buf128 b h memTaint t <==> valid_taint_buf128 b h' memTaint t)
+  [SMTPat (modifies p h h'); SMTPat (valid_taint_buf128 b h' memTaint t)]
